forcing_uip/def.v
@@ -1,0 +1,301 @@
+Set Primitive Projections.
+Set Universe Polymorphism.
+
+Inductive seq {A : Type} (x : A) : A -> SProp := srefl : seq x x.
+
+Notation "x ≡ y" := (seq x y) (at level 70).
+
+Axiom J_seq : forall (A : Type) (x : A) (P : forall y, x ≡ y -> Type),
+  P x (srefl _) -> forall y e, P y e.
+
+Inductive sFalse : SProp :=.
+
+Axiom ℙ@{} : Set.
+Axiom le₀@{} : ℙ -> ℙ -> Set.
+
+Definition le p q := forall r, le₀ q r -> le₀ p r.
+
+Definition le_id {p} : le p p := fun r k => k.
+Definition le_cmp {p q r} (α : le p q) (β : le q r) : le p r := fun r k => α r (β r k).
+
+Notation "p ≤ q" := (le p q) (at level 70, no associativity).
+Notation "'!'" := (@le_id _).
+Notation "α ∘ β" := (@le_cmp _ _ _ β α) (at level 35).
+
+Notation "α · x" := (fun r β => x r (α ∘ β)) (at level 40).
+
+Record TYPE@{i} (p : ℙ) := mkTYPE {
+  typ : forall q (α : q ≤ p), Type@{i};
+  rel : (forall q (α : q ≤ p), typ q α) -> SProp;
+}.
+
+Arguments typ {_}.
+Arguments rel {_}.
+
+Definition El {p : ℙ} (A : forall q (α : q ≤ p), TYPE q) :=
+  forall q (α : q ≤ p), (A q α).(typ) q !.
+
+Definition cast : forall {p : ℙ}
+  (A : forall q (α : q ≤ p), TYPE q)
+  (Aε : forall q (α : q ≤ p),
+    forall r (β : r ≤ q), (A q α).(typ) r β ≡ (A r (α ∘ β)).(typ) r !)
+  {q} (α : q ≤ p) {r} (β : r ≤ q), (A r (α ∘ β)).(typ) r ! -> (A q α).(typ) r β.
+Proof.
+refine (fun p A Aε q α r β x => _).
+refine (J_seq _ _ (fun X _ => X -> (A q α).(typ) r β) (fun r => r) _ (Aε q α r β) x).
+Defined.
+
+(*
+Definition Elε {p : ℙ}
+  (A : forall q (α : q ≤ p), TYPE q)
+  (Aε : forall q (α : q ≤ p),
+    forall r (β : r ≤ q), (A q α).(typ) r β ≡ (A r (α ∘ β)).(typ) r !)
+*)
+
+Definition K p : forall
+  (A : forall q (α : q ≤ p), TYPE q)
+  (Aε : forall q (α : q ≤ p),
+    forall r (β : r ≤ q), (A q α).(typ) r β ≡ (A r (α ∘ β)).(typ) r !)
+  (B : forall q (α : q ≤ p), TYPE q)
+  (Bε : forall q (α : q ≤ p),
+    forall r (β : r ≤ q), (B q α).(typ) r β ≡ (B r (α ∘ β)).(typ) r !)
+  (x : El A)
+  (xε : forall q (α : q ≤ p), (A q α).(rel) (fun r (β : r ≤ q) => cast A Aε α β (x r (α ∘ β))))
+  (y : El B)
+  (yε : forall q (α : q ≤ p), (B q α).(rel) (fun r (β : r ≤ q) => cast B Bε α β (y r (α ∘ β))))
+  q (α : q ≤ p)
+,
+(A q α).(typ) q !.
+Proof.
+refine (fun A Aε B Bε x xε y yε q α => x q α).
+Defined.
+
+Definition Kε p : forall
+  (A : forall q (α : q ≤ p), TYPE q)
+  (Aε : forall q (α : q ≤ p),
+    forall r (β : r ≤ q), (A q α).(typ) r β ≡ (A r (α ∘ β)).(typ) r !)
+  (B : forall q (α : q ≤ p), TYPE q)
+  (Bε : forall q (α : q ≤ p),
+    forall r (β : r ≤ q), (B q α).(typ) r β ≡ (B r (α ∘ β)).(typ) r !)
+  (x : El A)
+  (xε : forall q (α : q ≤ p), (A q α).(rel) (fun r (β : r ≤ q) => cast A Aε α β (x r (α ∘ β))))
+  (y : El B)
+  (yε : forall q (α : q ≤ p), (B q α).(rel) (fun r (β : r ≤ q) => cast B Bε α β (y r (α ∘ β))))
+  q (α : q ≤ p)
+,
+  (A q α).(rel) (fun r β => cast A Aε α β (K p A Aε B Bε x xε y yε r (α ∘ β))).
+Proof.
+intros.
+apply xε.
+Defined.
+
+Definition Arr p : forall
+  (A : forall q (α : q ≤ p), TYPE q)
+  (Aε : forall q (α : q ≤ p),
+    forall r (β : r ≤ q), (A q α).(typ) r β ≡ (A r (α ∘ β)).(typ) r !)
+  (B : forall q (α : q ≤ p), TYPE q)
+  (Bε : forall q (α : q ≤ p),
+    forall r (β : r ≤ q), (B q α).(typ) r β ≡ (B r (α ∘ β)).(typ) r !)
+  q (α : q ≤ p), TYPE q.
+Proof.
+unshelve refine (fun A Aε B Bε q α => mkTYPE _ _ _).
++ unshelve refine (fun r β =>
+  forall
+  (x : forall s (γ : s ≤ r), (A s (α ∘ β ∘ γ)).(typ) s !)
+  (xε : forall s (γ : s ≤ r), (A s (α ∘ β ∘ γ)).(rel)
+    (fun t (δ : t ≤ s) => cast A Aε (α ∘ β ∘ γ) δ (x t (γ ∘ δ))))
+  ,
+  (B r (α ∘ β)).(typ) r !).
++ unshelve refine (fun f =>
+  forall
+  (x : forall r (β : r ≤ q), (A r (α ∘ β)).(typ) r !)
+  (xε : forall r (β : r ≤ q), (A r (α ∘ β)).(rel)
+    (fun s (γ : s ≤ r) => cast A Aε (α ∘ β) γ (x s (β ∘ γ))))
+  ,
+  (B q α).(rel) (fun r β =>
+    cast B Bε α _ (f r β (β · x) (β · xε)))
+).
+Defined.
+
+Definition Arrε p : forall
+  (A : forall q (α : q ≤ p), TYPE q)
+  (Aε : forall q (α : q ≤ p),
+    forall r (β : r ≤ q), (A q α).(typ) r β ≡ (A r (α ∘ β)).(typ) r !)
+  (B : forall q (α : q ≤ p), TYPE q)
+  (Bε : forall q (α : q ≤ p),
+    forall r (β : r ≤ q), (B q α).(typ) r β ≡ (B r (α ∘ β)).(typ) r !)
+  q (α : q ≤ p) r (β : r ≤ q),
+  (Arr p A Aε B Bε q α).(typ) r β ≡ (Arr p A Aε B Bε r (α ∘ β)).(typ) r !.
+Proof.
+reflexivity.
+Defined.
+
+Definition Prod p : forall
+  (A : forall q (α : q ≤ p), TYPE q)
+  (Aε : forall q (α : q ≤ p),
+    forall r (β : r ≤ q), (A q α).(typ) r β ≡ (A r (α ∘ β)).(typ) r !)
+  (B : forall q (α : q ≤ p)
+    (x : forall r (β : r ≤ q), (A r (α ∘ β)).(typ) r !)
+    (xε : forall r (β : r ≤ q), (A r (α ∘ β)).(rel)
+      (fun s (γ : s ≤ r) => cast A Aε (α ∘ β) γ (x s (β ∘ γ)))),
+    TYPE q)
+  (Bε : forall q (α : q ≤ p)
+    (x : forall r (β : r ≤ q), (A r (α ∘ β)).(typ) r !)
+    (xε : forall r (β : r ≤ q), (A r (α ∘ β)).(rel)
+      (fun s (γ : s ≤ r) => cast A Aε (α ∘ β) γ (x s (β ∘ γ)))),
+    forall r (β : r ≤ q),
+      (B q α x xε).(typ) r β ≡ (B r (α ∘ β) (β · x) (β · xε)).(typ) r !
+  )
+  q (α : q ≤ p), TYPE q.
+Proof.
+unshelve refine (fun A Aε B Bε q α => mkTYPE _ _ _).
++ unshelve refine (fun r β =>
+  forall
+  (x : forall s (γ : s ≤ r), (A s (α ∘ β ∘ γ)).(typ) s !)
+  (xε : forall s (γ : s ≤ r), (A s (α ∘ β ∘ γ)).(rel)
+    (fun t (δ : t ≤ s) => cast A Aε (α ∘ β ∘ γ) δ (x t (γ ∘ δ))))
+  ,
+  (B r (α ∘ β) x xε).(typ) r !).
++ unshelve refine (fun f =>
+  forall
+  (x : forall r (β : r ≤ q), (A r (α ∘ β)).(typ) r !)
+  (xε : forall r (β : r ≤ q), (A r (α ∘ β)).(rel)
+    (fun s (γ : s ≤ r) => cast A Aε (α ∘ β) γ (x s (β ∘ γ))))
+  ,
+  (B q α x xε).(rel) _
+).
+unshelve refine (fun r β => @cast q
+  (fun s (γ : s ≤ q) => B s (α ∘ γ) (γ · x) (γ · xε))
+  (fun s (γ : s ≤ q) => Bε s (α ∘ γ) (γ · x) (γ · xε))
+  _ ! _ β (f r _ (β · x) (β · xε))).
+Defined.
+
+Definition Prodε p : forall
+  (A : forall q (α : q ≤ p), TYPE q)
+  (Aε : forall q (α : q ≤ p),
+    forall r (β : r ≤ q), (A q α).(typ) r β ≡ (A r (α ∘ β)).(typ) r !)
+  (B : forall q (α : q ≤ p)
+    (x : forall r (β : r ≤ q), (A r (α ∘ β)).(typ) r !)
+    (xε : forall r (β : r ≤ q), (A r (α ∘ β)).(rel)
+      (fun s (γ : s ≤ r) => cast A Aε (α ∘ β) γ (x s (β ∘ γ)))),
+    TYPE q)
+  (Bε : forall q (α : q ≤ p)
+    (x : forall r (β : r ≤ q), (A r (α ∘ β)).(typ) r !)
+    (xε : forall r (β : r ≤ q), (A r (α ∘ β)).(rel)
+      (fun s (γ : s ≤ r) => cast A Aε (α ∘ β) γ (x s (β ∘ γ)))),
+    forall r (β : r ≤ q),
+      (B q α x xε).(typ) r β ≡ (B r (α ∘ β) (β · x) (β · xε)).(typ) r !
+  )
+  q (α : q ≤ p) r (β : r ≤ q),
+  (Prod p A Aε B Bε q α).(typ) r β ≡ (Prod p A Aε B Bε r (α ∘ β)).(typ) r !.
+Proof.
+reflexivity.
+Defined.
+
+Definition Typeᶠ p : forall q (α : q ≤ p), TYPE q.
+Proof.
+unshelve econstructor.
++ refine (fun r β => TYPE r).
++ unshelve refine (fun A =>
+  forall r (β : r ≤ q) s (γ : s ≤ r),
+    (A r β).(typ) s γ ≡ (A s (β ∘ γ)).(typ) s !).
+Defined.
+
+Definition Typeε p :
+  forall q (α : q ≤ p) r (β : r ≤ q),
+    (Typeᶠ p q α).(typ) r β ≡ (Typeᶠ p r (α ∘ β)).(typ) r !.
+Proof.
+reflexivity.
+Defined.
+
+Inductive sumᶠ p
+  (A : forall q (α : q ≤ p), TYPE q)
+  (Aε : forall q (α : q ≤ p),
+    forall r (β : r ≤ q), (A q α).(typ) r β ≡ (A r (α ∘ β)).(typ) r !)
+  (B : forall q (α : q ≤ p), TYPE q)
+  (Bε : forall q (α : q ≤ p),
+    forall r (β : r ≤ q), (B q α).(typ) r β ≡ (B r (α ∘ β)).(typ) r !) :=
+| inlᶠ : forall
+  (x : El A)
+  (xε : forall q (α : q ≤ p), (A q α).(rel) (fun r (β : r ≤ q) => cast A Aε α β (x r (α ∘ β)))),
+  sumᶠ p A Aε B Bε
+| inrᶠ : forall
+  (y : El B)
+  (yε : forall q (α : q ≤ p), (B q α).(rel) (fun r (β : r ≤ q) => cast B Bε α β (y r (α ∘ β)))),
+  sumᶠ p A Aε B Bε
+.
+
+Inductive sumε p
+  (A : forall q (α : q ≤ p), TYPE q)
+  (Aε : forall q (α : q ≤ p),
+    forall r (β : r ≤ q), (A q α).(typ) r β ≡ (A r (α ∘ β)).(typ) r !)
+  (B : forall q (α : q ≤ p), TYPE q)
+  (Bε : forall q (α : q ≤ p),
+    forall r (β : r ≤ q), (B q α).(typ) r β ≡ (B r (α ∘ β)).(typ) r !)
+  : (forall q α, sumᶠ q (α · A) (α · Aε) (α · B) (α · Bε)) -> SProp :=
+| inlε : forall
+  (x : El A)
+  (xε : forall q (α : q ≤ p), (A q α).(rel) (fun r (β : r ≤ q) => cast A Aε α β (x r (α ∘ β)))),
+  sumε p A Aε B Bε (fun q α => inlᶠ q (α · A) (α · Aε) (α · B) (α · Bε) (α · x) (α · xε))
+| inrε : forall
+  (y : El B)
+  (yε : forall q (α : q ≤ p), (B q α).(rel) (fun r (β : r ≤ q) => cast B Bε α β (y r (α ∘ β)))),
+  sumε p A Aε B Bε (fun q α => inrᶠ q (α · A) (α · Aε) (α · B) (α · Bε) (α · y) (α · yε))
+.
+
+Definition sum_elim p : forall
+  (A : forall q (α : q ≤ p), TYPE q)
+  (Aε : forall q (α : q ≤ p),
+    forall r (β : r ≤ q), (A q α).(typ) r β ≡ (A r (α ∘ β)).(typ) r !)
+  (B : forall q (α : q ≤ p), TYPE q)
+  (Bε : forall q (α : q ≤ p),
+    forall r (β : r ≤ q), (B q α).(typ) r β ≡ (B r (α ∘ β)).(typ) r !)
+  (P : forall q (α : q ≤ p)
+    (v : forall r (β : r ≤ q), sumᶠ r (α ∘ β · A) (α ∘ β · Aε) (α ∘ β · B) (α ∘ β · Bε))
+    (vε : forall r (β : r ≤ q), sumε r (α ∘ β · A) (α ∘ β · Aε) (α ∘ β · B) (α ∘ β · Bε)
+      (fun s (γ : s ≤ r) => (v s (β ∘ γ)))),
+    TYPE q)
+  (Pε : forall q (α : q ≤ p)
+    (v : forall r (β : r ≤ q), sumᶠ r (α ∘ β · A) (α ∘ β · Aε) (α ∘ β · B) (α ∘ β · Bε))
+    (vε : forall r (β : r ≤ q), sumε r (α ∘ β · A) (α ∘ β · Aε) (α ∘ β · B) (α ∘ β · Bε)
+      (fun s (γ : s ≤ r) => (v s (β ∘ γ)))),
+    forall r (β : r ≤ q),
+      (P q α v vε).(typ) r β ≡ (P r (α ∘ β) (β · v) (β · vε)).(typ) r !
+  )
+  (ul : forall q (α : q ≤ p)
+    (x : forall r (β : r ≤ q), (A r (α ∘ β)).(typ) r !)
+    (xε : forall r (β : r ≤ q), (A r (α ∘ β)).(rel)
+      (fun s (γ : s ≤ r) => cast A Aε (α ∘ β) γ (x s (β ∘ γ)))),
+    (P q α
+      (fun r β => inlᶠ r (α ∘ β · A) (α ∘ β · Aε) _ _ (β · x) (β · xε))
+      (fun r β => inlε r (α ∘ β · A) (α ∘ β · Aε) _ _ (β · x) (β · xε))).(typ) q !)
+  (ulε : forall q (α : q ≤ p)
+    (x : forall r (β : r ≤ q), (A r (α ∘ β)).(typ) r !)
+    (xε : forall r (β : r ≤ q), (A r (α ∘ β)).(rel)
+      (fun s (γ : s ≤ r) => cast A Aε (α ∘ β) γ (x s (β ∘ γ)))),
+    (P q α
+      (fun r β => inlᶠ r (α ∘ β · A) (α ∘ β · Aε) _ _ (β · x) (β · xε))
+      (fun r β => inlε r (α ∘ β · A) (α ∘ β · Aε) _ _ (β · x) (β · xε))).(rel)
+        (fun r β =>
+          @cast q
+            (fun s (γ : s ≤ q) => P s (α ∘ γ)
+              (fun t (δ : t ≤ s) => inlᶠ t _ _ _ _ (γ ∘ δ · x) (γ ∘ δ · xε)) (fun t (δ : t ≤ s) => inlε t (α ∘ γ ∘ δ · A) (α ∘ γ ∘ δ · Aε) _ _ (γ ∘ δ · x) (γ ∘ δ · xε)))
+            (fun s (γ : s ≤ q) => Pε s (α ∘ γ)
+              (fun t (δ : t ≤ s) => inlᶠ t _ _ _ _ (γ ∘ δ · x) (γ ∘ δ · xε)) (fun t (δ : t ≤ s) => inlε t (α ∘ γ ∘ δ · A) (α ∘ γ ∘ δ · Aε) _ _ (γ ∘ δ · x) (γ ∘ δ · xε)))
+          q ! r β (ul r (α ∘ β) (β · x) (β · xε))
+        ))
+  (ur : forall q (α : q ≤ p)
+    (y : forall r (β : r ≤ q), (B r (α ∘ β)).(typ) r !)
+    (yε : forall r (β : r ≤ q), (B r (α ∘ β)).(rel)
+      (fun s (γ : s ≤ r) => cast B Bε (α ∘ β) γ (y s (β ∘ γ)))),
+    (P q α
+      (fun r β => inrᶠ r (α ∘ β · A) (α ∘ β · Aε) _ _ (β · y) (β · yε))
+      (fun r β => inrε r (α ∘ β · A) (α ∘ β · Aε) _ _ (β · y) (β · yε))).(typ) q !)
+  (b : forall q (α : q ≤ p), sumᶠ q (α · A) (α · Aε) (α · B) (α · Bε))
+  (bε : forall q (α : q ≤ p), sumε q (α · A) (α · Aε) (α · B) (α · Bε) (α · b))
+ q (α : q ≤ p)
+,
+  (P q α (α · b) (α · bε)).(typ) q !.
+Proof.
+intros.
+Admitted.
